theories/prob_eff_lang/probblaze/examples/DH_KE/dhke_channel_lazy_real_other.v
@@ -7,7 +7,7 @@ From clutch.prob_eff_lang.probblaze Require Import logic primitive_laws proofmod
   spec_rules spec_ra 
   class_instances. 
 From clutch.prob_eff_lang.probblaze Require Import tactics.
-From clutch.prob_eff_lang.probblaze Require Import def_dhke.
+From clutch.prob_eff_lang.probblaze Require Import def_dhke dhke_common.
 From clutch.prob_eff_lang.probblaze Require Import sem_types sem_row sem_sig sem_judgement sem_def. 
 
 Import fingroup.
@@ -150,12 +150,7 @@ Section handlee_verification.
         iSplitL; [|by iIntros "!>" (??) "H"; iApply "H"].
         iLeft. 
         iExists _,_,_.
-        iSplitL.
-        { iMod (inv_acc with "Hinvta") as "([>Htok | >#Hfrac'] & Hclose)"; try done.
-          - iModIntro. iLeft.
-            iIntros. iFrame. iMod ("Hclose" with "[$]") as "_". iFrame "#". 
-            by iModIntro.
-          - iModIntro. iRight. by iMod ("Hclose" with "[$]") as "_". }
+        iSplitL; first (iApply send_upd; by iFrame "#").
         iSplit; first ( do 2 (iSplit; try (iPureIntro; done))).
         iModIntro.
         iApply brel_value. iIntros "$ !>"...
@@ -197,14 +192,7 @@ Section handlee_verification.
         iSplitL; [|by iIntros "!>" (??) "H"; iApply "H"].
         iLeft.
         iExists _,_,_.
-        iSplitL.
-        { iMod (inv_acc with "Hinvta") as "([>Htok | >#Hfrac'] & Hclose)"; try done.
-          - iModIntro. iLeft.
-            iIntros. iFrame. iMod ("Hclose" with "[$]") as "_". iFrame "#". 
-            by iModIntro. 
-          - iModIntro. iRight. iFrame "#".
-            iApply "Hclose". iNext.
-            by iRight. }
+        iSplitL; first (iApply send_upd; by iFrame "#").
         iSplit; first (iSplit; try (iPureIntro; done)).
         iModIntro.
         iApply brel_value. iIntros "$ !>"...
@@ -216,11 +204,10 @@ Section handlee_verification.
         iRight.
         do 2 (iSplit; try (iPureIntro; done)).
         iModIntro.
-        iSplitL.
+        iSplitL...
         
         (* Recv bob = None *)
-        + iApply brel_value. iIntros "$ !>"...
-          iDestruct ("Hcont" with "Hnone") as "Hkk".
+        + iDestruct ("Hcont" with "Hnone") as "Hkk".
           iApply (brel_exhaustion with "[$]"); [done|done|].
           iApply "IH".
           
@@ -276,12 +263,7 @@ Section handlee_verification.
         iSplitL; [|by iIntros "!>" (??) "H"; iApply "H"].
         iRight. 
         iExists _,_.
-        iSplitL.
-        { iMod (inv_acc with "Hinvtb") as "([>Htok | >#Hfrac'] & Hclose)"; try done.
-          - iModIntro. iLeft.
-            iIntros. iFrame. iMod ("Hclose" with "[$]") as "_". iFrame "#". 
-            by iModIntro. 
-          - iModIntro. iRight. by iMod ("Hclose" with "[$]") as "_". }
+        iSplitL; first (iApply send_upd; by iFrame "#").
         iSplit; first ( do 2 (iSplit; try (iPureIntro; done))).
         iModIntro.
         iApply brel_value. iIntros "$ !>"...
@@ -308,12 +290,7 @@ Section handlee_verification.
         iSplitL; [|by iIntros "!>" (??) "H"; iApply "H"].
         iRight.
         iExists _,_.
-        iSplitL.
-        { iMod (inv_acc with "Hinvtb") as "([>Htok | >#Hfrac'] & Hclose)"; try done.
-          - iModIntro. iLeft.
-            iIntros. iFrame. iMod ("Hclose" with "[$]") as "_". iFrame "#". 
-            by iModIntro. 
-          - iModIntro. iRight. by iMod ("Hclose" with "[$]") as "_". }
+        iSplitL; first (iApply send_upd; by iFrame "#").
         iSplit; first ( do 2 (iSplit; try (iPureIntro; done))).
         
         iModIntro. 
