theories/prob_eff_lang/probblaze/examples/DH_KE/dhke_common.v
@@ -1,0 +1,36 @@
+From iris.proofmode Require Import base.
+From iris.base_logic.lib Require Import  na_invariants.
+From iris.algebra Require Export agree excl auth frac excl_auth.
+From iris.algebra.lib Require Export dfrac_agree.
+From clutch.prob_eff_lang.probblaze Require Import logic.
+
+Ltac label_not_in_singleton Hdl := 
+  apply NoDup_cons_1_1;
+  eapply submseteq_NoDup; last exact Hdl;
+  solve_submseteq. 
+
+Section lemmas.
+  Context `{!probblazeRGS Σ}.
+  Context `{!inG Σ (exclR unitO), !inG Σ dfracO, !inG Σ (dfrac_agreeR valO)}.
+
+  Definition token γ := own γ (Excl ()).
+
+  Lemma send_upd P n γtok γfrac :
+    P ∗
+    invariants.inv n (token γtok ∨ own γfrac DfracDiscarded) ⊢
+    (|={⊤,⊤ ∖ ↑n}=>
+       (own γfrac DfracDiscarded ={⊤ ∖ ↑n,⊤}=∗ token γtok ∗ P)
+        ∨ (|={⊤ ∖ ↑n,⊤}=> own γfrac DfracDiscarded)).
+  Proof. 
+    iIntros "(HP&#Hinv)".
+    iMod (inv_acc with "Hinv") as "([>Htok | >#Hfrac] & Hclose)"; try done.
+    - iModIntro. iLeft.
+      iIntros. iFrame. iMod ("Hclose" with "[$]") as "_". 
+      by iModIntro. 
+    - iModIntro. iRight. iFrame "#".
+      iApply "Hclose". iNext.
+      by iRight.
+  Qed. 
+
+End lemmas.
+
